για πραξη :α :β 
δειξε(δυναμη :α + :β 2)
τελος

για πραξη2 :α :β 
δειξε(δυναμη :α - :β 2)
τελος

για πραξη3 :α :β 
δειξε(δυναμη :α 2) + 2 * :α * :β + (δυναμη :β 2)
τελος

για πραξη4 :α :β
δειξε(δυναμη :α 2) - 2 * :α * :β + (δυναμη :β 2)
τελος

για πραξη5 :α :β
δειξε(δυναμη :α 2) - (δυναμη :β 2)
τελος

για πραξη6 :α :β
δειξε(:α + :β) * (:α - :β)
τελος

για πραξη7 :α :β
δειξε(δυναμη :α + :β 3)
τελος

για πραξη8 :α :β
δειξε(δυναμη :α - :β 3)
τελος

για πραξη9 :α :β
δειξε(δυναμη :α 3) + 3 * (δυναμη :α 2) * :β + 3 * :α * (δυναμη :β 2) + (δυναμη :β 3)
τελος

για πραξη10 :α :β
δειξε(δυναμη :α 3) - 3 * (δυναμη :α 2) * :β + 3 * :α * (δυναμη :β 2) - (δυναμη :β 3)
τελος

για πραξη11 :α :β
δειξε(δυναμη :α 3) + (δυναμη :β 3)
τελος

για πραξη12 :α :β
δειξε(δυναμη :α 3) - (δυναμη :β 3)
τελος

για πραξη13 :α :β
δειξε(:α + :β) * ((δυναμη :α 2 - :α * :β + (δυναμη :β 2))
τελος

για πραξη14 :α :β
δειξε(:α - :β) * [δυναμη :α 2 + :α * :β + (δυναμη :β 2)
